Isabelle/Composition.thy
@@ -1,5 +1,5 @@
 theory Composition
-imports ComposableGC "/home/nano/Documents/IO-Automata/Simulations"
+imports ComposableGC "/home/nano/Documents/IO-Automata/Simulations" "~~/src/HOL/Eisbach/Eisbach_Tools"
 begin
 
 datatype ('a,'c,'l) comp_action = 
@@ -44,7 +44,7 @@ fun rn3 where
 | "rn3 (ToNext s) = Some (cgc_action.ToNext s)"
 
 definition initial where
-  "initial \<equiv> cgc_ioa\<lparr>start := {\<lparr>propCmd = {}, learned = \<lambda> p . None, fromPrev = {\<bottom>}, toNext = {} \<rparr>}\<rparr>"
+  "initial \<equiv> cgc_ioa\<lparr>start := {\<lparr>propCmd = {}, learned = \<lambda> p . {}, fromPrev = {\<bottom>}, toNext = {} \<rparr>}\<rparr>"
 
 definition composition where
   "composition \<equiv> hide ((rename initial rn1) \<parallel> (rename cgc_ioa rn2)) {a . \<exists> s . a = Switch s}"
@@ -54,17 +54,28 @@ definition spec where
 
 definition inv1 where
   "inv1 r \<equiv> let r1 = fst r; r2 = snd r in
-    (\<forall> s \<in> cgc_state.fromPrev r2 . \<forall> l . 
-      case cgc_state.learned r1 l of Some s' \<Rightarrow> s' \<preceq> s | None \<Rightarrow> True)"
+    (\<forall> s \<in> cgc_state.fromPrev r2 . \<forall> l . \<forall> s' \<in> learned r1 l . s' \<preceq> s)"
 
 definition inv2 where
   "inv2 r \<equiv> let r1 = fst r; r2 = snd r in 
     cgc_state.fromPrev r2 = cgc_state.toNext r1"
 
+definition inv3 where
+  "inv3 r \<equiv> let r1 = fst r; r2 = snd r in
+    cgc_state.fromPrev r1 = {\<bottom>}"
+
+definition inv4 where
+  "inv4 r \<equiv> let r1 = fst r; r2 = snd r in
+    \<forall> l . \<forall> s \<in> learned r2 l . \<exists> s' \<in> cgc_state.fromPrev r2 . s' \<preceq> s"
+
+definition inv5 where
+  "inv5 r \<equiv> let r1 = fst r; r2 = snd r in
+    \<forall> s \<in> cgc_state.toNext r2 . \<exists> s' \<in> cgc_state.fromPrev r2 . s' \<preceq> s"
+
 lemmas defs1 = composition_def par2_def asig_comp2_def cgc_ioa_def rename_def cgc_start_def
     rename_set_def cgc_asig_def is_trans_def actions_def cgc_trans_def initial_def hide_def propose_def learn_def fromPrev_def toNext_def
     hide_asig_def externals_def cgc_start_def spec_def
-     
+
 lemmas ref_defs = refines_def actions_def trace_def schedule_def filter_act_def
 
 lemma inv2:"invariant composition inv2"
@@ -82,12 +93,52 @@ apply (rule invariantI)
   apply(auto simp add:defs1 inv1_def inv2_def non_trivial_def)
 done
 
+lemma inv3:"invariant composition inv3"
+apply (rule invariantI)
+  apply(simp add:defs1 inv3_def)
+  apply(case_tac "a")
+  apply(auto simp add:defs1 inv3_def)
+done
+
+lemma inv4:"invariant composition inv4"
+apply (rule invariantI)
+  apply(simp add:defs1 inv4_def)
+  apply(case_tac "a")
+  apply(thin_tac "reachable composition s")
+  apply(auto simp add:defs1 inv4_def non_trivial_def less_eq_def)
+done
+
+lemma inv5:"invariant composition inv5"
+apply (rule invariantI)
+  apply(simp add:defs1 inv5_def)
+  apply(case_tac "a")
+  apply(thin_tac "reachable composition s")
+  apply(auto simp add:defs1 inv5_def non_trivial_def less_eq_def)
+done
+
+lemmas inv11 = inv1[simplified invariant_def]
+thm inv11[split_format(complete)]
+lemmas invs[simplified invariant_def, rule_format] = inv1 inv2
+
+lemma l1:
+  assumes "s\<^sub>0 \<preceq> s\<^sub>1" and "s\<^sub>2 = s\<^sub>1 \<star> cs"
+  shows "compat2 s\<^sub>0 s\<^sub>2"
+  using assms
+by (metis less_eq_def local.compat2_def local.trans) 
+
 abbreviation refmap where
   "refmap r \<equiv> let r1 = fst r; r2 = snd r in 
     \<lparr>cgc_state.propCmd = propCmd r1 \<union> propCmd r2, 
-      cgc_state.learned = (\<lambda> l . case learned r2 l of None \<Rightarrow> learned r1 l | _ \<Rightarrow> learned r2 l), 
+      cgc_state.learned = (\<lambda> l . learned r1 l \<union> learned r2 l),
       cgc_state.fromPrev = {\<bottom>}, 
       toNext = cgc_state.toNext r2\<rparr>"
+
+method my_allE for y :: 'a =
+(match premises in I [thin]: "\<forall> x :: 'a. ?Q x" \<Rightarrow>
+  \<open>rule allE [where x = y, OF I ]\<close>)
+
+method print_inv =
+  match invs in M [thin] :"\<And> s . reachable composition s \<Longrightarrow> ?Inv" \<Rightarrow> \<open>print_fact M\<close>
 
 lemma refok:"is_ref_map refmap composition spec"
 apply(simp add:is_ref_map_def, rule conjI; clarify)
@@ -97,30 +148,78 @@ apply(simp add:is_ref_map_def, rule conjI; clarify)
    apply(rule_tac x="refmap (a,b)" in exI)
    apply(rule_tac x="[(Propose1 x1,refmap (aa,ba))]" in exI)
    apply(simp add:defs1 ref_defs)
-   apply(simp add:fun_eq_iff, rule allI) 
-   apply(case_tac "learned ba x", force+)
 
    apply(thin_tac "reachable composition (a, b)")
    apply(rule_tac x="refmap (a,b)" in exI)
    apply(rule_tac x="[(Propose2 x2,refmap (aa,ba))]" in exI)
    apply(simp add:defs1 ref_defs)
-   apply(simp add:fun_eq_iff, rule allI) 
-   apply(case_tac "learned b x", auto)
 
    prefer 3
    apply(thin_tac "reachable composition (a, b)")
    apply(rule_tac x="refmap (a,b)" in exI)
    apply(rule_tac x="[]" in exI)
    apply(simp add:defs1 ref_defs)
-   apply auto
-   apply(simp add:fun_eq_iff, rule allI) 
-   apply(case_tac "learned b x", auto)
 
-  apply(thin_tac "reachable composition (a, b)")
    apply(rule_tac x="refmap (a,b)" in exI)
    apply(rule_tac x="[(Learn1 x31 x32,refmap (aa,ba))]" in exI)
-   apply(simp add:defs1 ref_defs)
-sorry
+   apply(frule_tac inv1[simplified invariant_def, rule_format])
+   apply(frule_tac inv3[simplified invariant_def, rule_format])
+   apply(frule_tac inv2[simplified invariant_def, rule_format])
+   apply(frule_tac inv4[simplified invariant_def, rule_format])
+   apply(frule_tac inv5[simplified invariant_def, rule_format])
+   apply(thin_tac "reachable composition (a,b)")
+   proof -
+    fix r1 r2 l r1' r2' s
+    assume learn:"(r1, r2) \<midarrow>Learn1 s l\<midarrow>composition\<longrightarrow> (r1', r2')" and inv1:"inv1 (r1, r2)" and inv2:"inv2 (r1, r2)" and inv3:"inv3 (r1,r2)" and inv4:"inv4 (r1,r2)"
+    and inv5:"inv5 (r1,r2)"
+    show "refines (refmap (r1, r2), [(Learn1 s l, refmap (r1', r2'))]) (r1, r2) (Learn1 s l) (r1', r2') spec refmap"
+    proof -
+      from learn have 1:"learn l s r1 r1'" and 2:"r2 = r2'"
+        by (auto simp add: defs1)
+      have "learn l s (refmap (r1, r2)) (refmap (r1',r2'))"
+      proof -
+        have "s \<in> non_trivial (refmap (r1, r2))" using 1 inv3 
+          by (auto simp add:learn_def inv3_def non_trivial_def)
+        moreover
+        have "cgc_state.fromPrev (refmap (r1, r2)) \<noteq> {}" using inv3
+          by (auto simp add:inv3_def)
+        moreover 
+        have "let learned1 = learned (refmap (r1, r2)) in (refmap (r1', r2')) = (refmap (r1, r2))\<lparr>learned := (learned1(l := learned1 l \<union> {s}))\<rparr>"
+          using 1 2
+          by (auto simp add:learn_def fun_eq_iff)
+        moreover 
+        have "\<forall> l . \<forall> s' \<in> learned (refmap (r1, r2)) l . compat2 s' s"
+        proof auto
+          fix l s'
+          assume "s' \<in> learned r1 l"
+          thus "compat2 s' s" using 1 by (simp add:learn_def)
+        next
+          fix l s'
+          assume 3:"s' \<in> learned r2 l"
+          with this obtain s'' where 4:"s'' \<preceq> s'" and 5:"s'' \<in> cgc_state.fromPrev r2" using inv4
+            by (auto simp add:inv4_def)
+          moreover
+          have "s \<preceq> s''" using 5 inv1 inv2 1 by (auto simp add:inv2_def inv1_def learn_def)
+          ultimately
+          show "compat2 s' s" using l1
+            by (metis compat_sym less_eq_def) 
+        qed
+        moreover
+        have "\<forall> s' \<in> cgc_state.toNext (refmap (r1, r2)) . s \<preceq> s'"
+        proof auto
+          fix s'
+          assume "s' \<in> cgc_state.toNext r2"
+          with this obtain s'' where 4:"s'' \<preceq> s'" and 5:"s'' \<in> cgc_state.fromPrev r2" using inv5
+            by (auto simp add:inv5_def)
+          have 6:"s \<preceq> s''" using 5 inv1 inv2 1 by (auto simp add:inv2_def inv1_def learn_def)
+          show "s \<preceq> s'" using 4 6
+            by (metis pre_CStruct.trans)
+        qed
+        ultimately
+        show ?thesis by (auto simp add:learn_def)
+      qed
+      thus ?thesis by (auto simp add:defs1 ref_defs)
+    qed next
 
 lemma trace_incl:"traces composition \<subseteq> traces spec"
 apply(rule ref_map_soundness[of refmap])
